\begin{property}[Symétrie des coefficients binomiaux]
\label{binome:symetrie}
Soient $n \in \setNaturalNumbers$ et $k \in \integerIntervalCC{0}{n}$, alors 
\[
\binom{n}{k} = \binom{n}{n-k}
\]
\end{property}

\begin{proof}
Soient $n \in \setNaturalNumbers$ et $k \in \integerIntervalCC{0}{n}$, par définition
\[
\binom{n}{n-k} = \dfrac{n!}{(n-k)!(n-(n-k))!}= \dfrac{n!}{(n-k)!k!}
\]
car $(n-(n-k))= n-n+ k = k$. On a alors
\[
\lboxed{\displaystyle\binom{n}{n-k}} =\dfrac{n!}{k!(n-k)!} \rboxed{=\displaystyle\binom{n}{k}}
\]
\end{proof}